TAO_5_Quantifiable.thy
@@ -20,18 +20,10 @@ text{*
 subsection{* Type Class *}
 text{* \label{TAO_Quantifiable_Class} *}
 
-text{* Datatype of types for which quantification is defined: *}
-
-datatype var = \<nu>var (var\<nu>: \<nu>) | \<o>var (var\<o>: \<o>) | \<Pi>\<^sub>1var (var\<Pi>\<^sub>1: \<Pi>\<^sub>1)
-             | \<Pi>\<^sub>2var (var\<Pi>\<^sub>2: \<Pi>\<^sub>2) | \<Pi>\<^sub>3var (var\<Pi>\<^sub>3: \<Pi>\<^sub>3)
-
 text{* Type class for quantifiable types: *}
 
 class quantifiable = fixes forall :: "('a\<Rightarrow>\<o>)\<Rightarrow>\<o>" (binder "\<^bold>\<forall>" [8] 9)
-                       and qvar :: "'a\<Rightarrow>var"
-                       and varq :: "var\<Rightarrow>'a"
   assumes quantifiable_T8: "(w \<Turnstile> (\<^bold>\<forall> x . \<psi> x)) = (\<forall> x . (w \<Turnstile> (\<psi> x)))"
-      and varq_qvar_id: "varq (qvar x) = x"
 begin
   definition exists :: "('a\<Rightarrow>\<o>)\<Rightarrow>\<o>" (binder "\<^bold>\<exists>" [8] 9) where
     "exists \<equiv> \<lambda> \<phi> . \<^bold>\<not>(\<^bold>\<forall> x . \<^bold>\<not>\<phi> x)"
@@ -49,80 +41,50 @@ text{* \label{TAO_Quantifiable_Instantiation} *}
 instantiation \<nu> :: quantifiable
 begin
   definition forall_\<nu> :: "(\<nu>\<Rightarrow>\<o>)\<Rightarrow>\<o>" where "forall_\<nu> \<equiv> forall\<^sub>\<nu>"
-  definition qvar_\<nu> :: "\<nu>\<Rightarrow>var" where "qvar \<equiv> \<nu>var"
-  definition varq_\<nu> :: "var\<Rightarrow>\<nu>" where "varq \<equiv> var\<nu>"
   instance proof
     fix w :: i and \<psi> :: "\<nu>\<Rightarrow>\<o>"
     show "(w \<Turnstile> \<^bold>\<forall>x. \<psi> x) = (\<forall>x. (w \<Turnstile> \<psi> x))"
       unfolding forall_\<nu>_def using Semantics.T8_\<nu> .
-  next
-    fix x :: \<nu>
-    show "varq (qvar x) = x"
-      unfolding qvar_\<nu>_def varq_\<nu>_def by simp
   qed
 end
 
 instantiation \<o> :: quantifiable
 begin
   definition forall_\<o> :: "(\<o>\<Rightarrow>\<o>)\<Rightarrow>\<o>" where "forall_\<o> \<equiv> forall\<^sub>\<o>"
-  definition qvar_\<o> :: "\<o>\<Rightarrow>var" where "qvar \<equiv> \<o>var"
-  definition varq_\<o> :: "var\<Rightarrow>\<o>" where "varq \<equiv> var\<o>"
   instance proof
     fix w :: i and \<psi> :: "\<o>\<Rightarrow>\<o>"
     show "(w \<Turnstile> \<^bold>\<forall>x. \<psi> x) = (\<forall>x. (w \<Turnstile> \<psi> x))"
       unfolding forall_\<o>_def using Semantics.T8_\<o> .
-  next
-    fix x :: \<o>
-    show "varq (qvar x) = x"
-      unfolding qvar_\<o>_def varq_\<o>_def by simp
   qed
 end
 
 instantiation \<Pi>\<^sub>1 :: quantifiable
 begin
   definition forall_\<Pi>\<^sub>1 :: "(\<Pi>\<^sub>1\<Rightarrow>\<o>)\<Rightarrow>\<o>" where "forall_\<Pi>\<^sub>1 \<equiv> forall\<^sub>1"
-  definition qvar_\<Pi>\<^sub>1 :: "\<Pi>\<^sub>1\<Rightarrow>var" where "qvar \<equiv> \<Pi>\<^sub>1var"
-  definition varq_\<Pi>\<^sub>1 :: "var\<Rightarrow>\<Pi>\<^sub>1" where "varq \<equiv> var\<Pi>\<^sub>1"
   instance proof
     fix w :: i and \<psi> :: "\<Pi>\<^sub>1\<Rightarrow>\<o>"
     show "(w \<Turnstile> \<^bold>\<forall>x. \<psi> x) = (\<forall>x. (w \<Turnstile> \<psi> x))"
       unfolding forall_\<Pi>\<^sub>1_def using Semantics.T8_1 .
-  next
-    fix x :: \<Pi>\<^sub>1
-    show "varq (qvar x) = x"
-      unfolding qvar_\<Pi>\<^sub>1_def varq_\<Pi>\<^sub>1_def by simp
   qed
 end
 
 instantiation \<Pi>\<^sub>2 :: quantifiable
 begin
   definition forall_\<Pi>\<^sub>2 :: "(\<Pi>\<^sub>2\<Rightarrow>\<o>)\<Rightarrow>\<o>" where "forall_\<Pi>\<^sub>2 \<equiv> forall\<^sub>2"
-  definition qvar_\<Pi>\<^sub>2 :: "\<Pi>\<^sub>2\<Rightarrow>var" where "qvar \<equiv> \<Pi>\<^sub>2var"
-  definition varq_\<Pi>\<^sub>2 :: "var\<Rightarrow>\<Pi>\<^sub>2" where "varq \<equiv> var\<Pi>\<^sub>2"
   instance proof
     fix w :: i and \<psi> :: "\<Pi>\<^sub>2\<Rightarrow>\<o>"
     show "(w \<Turnstile> \<^bold>\<forall>x. \<psi> x) = (\<forall>x. (w \<Turnstile> \<psi> x))"
       unfolding forall_\<Pi>\<^sub>2_def using Semantics.T8_2 .
-  next
-    fix x :: \<Pi>\<^sub>2
-    show "varq (qvar x) = x"
-      unfolding qvar_\<Pi>\<^sub>2_def varq_\<Pi>\<^sub>2_def by simp
   qed
 end
 
 instantiation \<Pi>\<^sub>3 :: quantifiable
 begin
   definition forall_\<Pi>\<^sub>3 :: "(\<Pi>\<^sub>3\<Rightarrow>\<o>)\<Rightarrow>\<o>" where "forall_\<Pi>\<^sub>3 \<equiv> forall\<^sub>3"
-  definition qvar_\<Pi>\<^sub>3 :: "\<Pi>\<^sub>3\<Rightarrow>var" where "qvar \<equiv> \<Pi>\<^sub>3var"
-  definition varq_\<Pi>\<^sub>3 :: "var\<Rightarrow>\<Pi>\<^sub>3" where "varq \<equiv> var\<Pi>\<^sub>3"
   instance proof
     fix w :: i and \<psi> :: "\<Pi>\<^sub>3\<Rightarrow>\<o>"
     show "(w \<Turnstile> \<^bold>\<forall>x. \<psi> x) = (\<forall>x. (w \<Turnstile> \<psi> x))"
       unfolding forall_\<Pi>\<^sub>3_def using Semantics.T8_3 .
-  next
-    fix x :: \<Pi>\<^sub>3
-    show "varq (qvar x) = x"
-      unfolding qvar_\<Pi>\<^sub>3_def varq_\<Pi>\<^sub>3_def by simp
   qed
 end
 
